feat: Restored compilability after concatenating directory files

examples/scalaEquivalenceBenchmarkExamples/binSum.dfy
@@ -12,19 +12,19 @@ function length<T>(l: List<T>): nat
 // This tests the normalization function where the return type is changed
 
 
-function binSum(l1: List<bool>, l2: List<bool>, c: bool): List<bool>
+function binSumM(l1: List<bool>, l2: List<bool>, c: bool): List<bool>
   decreases length(l1) + length(l2)
   {
     match (l1, l2)
     case (Nil, Nil) => Nil
-    case (Cons(true, t1), Cons(false, t2)) => Cons(!c, binSum(t1, t2, c))
-    case (Cons(false, t1), Cons(true, t2)) => Cons(!c, binSum(t1, t2, c))
-    case (Cons(false, t1), Cons(false, t2)) => Cons(c, binSum(t1, t2, false))
-    case (Cons(true, t1), Cons(true, t2)) => Cons(c, binSum(t1, t2, true))
-    case (Cons(true, t1), Nil) => Cons(!c, binSum(t1, Nil, c))
-    case (Cons(false, t1), Nil) => Cons(c, binSum(t1, Nil, false))
-    case (Nil, Cons(true, t2)) => Cons(!c, binSum(t2, Nil, c))
-    case (Nil, Cons(false, t2)) => Cons(c, binSum(t2, Nil, false))
+    case (Cons(true, t1), Cons(false, t2)) => Cons(!c, binSumM(t1, t2, c))
+    case (Cons(false, t1), Cons(true, t2)) => Cons(!c, binSumM(t1, t2, c))
+    case (Cons(false, t1), Cons(false, t2)) => Cons(c, binSumM(t1, t2, false))
+    case (Cons(true, t1), Cons(true, t2)) => Cons(c, binSumM(t1, t2, true))
+    case (Cons(true, t1), Nil) => Cons(!c, binSumM(t1, Nil, c))
+    case (Cons(false, t1), Nil) => Cons(c, binSumM(t1, Nil, false))
+    case (Nil, Cons(true, t2)) => Cons(!c, binSumM(t2, Nil, c))
+    case (Nil, Cons(false, t2)) => Cons(c, binSumM(t2, Nil, false))
   }
 
 function norm(l1: List<bool>, l2: List<bool>, c: bool, res: List<bool>): int
@@ -37,15 +37,6 @@ function listToInt(l: List<bool>): int {
   }
 
 // CANDIDATE
-
-datatype List<T> = Nil | Cons(head: T, tail: List<T>)
-
-function length<T>(l: List<T>): nat
-  {
-  match l
-    case Nil => 0
-    case Cons(_, t) => 1 + length(t)
-  }
 
 function binSum(l1: List<bool>, l2: List<bool>, c: bool): List<bool>
   decreases length(l1) + length(l2)
