examples/scalaEquivalenceBenchmarkExamples/dup.dfy
@@ -3,10 +3,10 @@
 datatype List<T> = Nil | Cons(head: T, tail: List<T>)
 
 
-function dup<S, T>(n: int, s: S, t: T): List<(S, T)>
+function dupM<S, T>(n: int, s: S, t: T): List<(S, T)>
   decreases(if (n <= 0) then 0 else n) {
   if (n <= 0) then Nil
-  else Cons((s, t), dup(n - 1, s, t))
+  else Cons((s, t), dupM(n - 1, s, t))
 }
 
 function norm<S, T>(n: int, s: S, t: T, res: List<(S, T)>): List<(S, T)>
@@ -16,58 +16,44 @@ function norm<S, T>(n: int, s: S, t: T, res: List<(S, T)>): List<(S, T)>
 
 // CANDIDATE 1
 
-datatype List<T> = Nil | Cons(head: T, tail: List<T>)
-
-
-function dup<S, T>(n: int, s: S, t: T): List<(S, T)>
+function dup1<S, T>(n: int, s: S, t: T): List<(S, T)>
   decreases(if (n <= 0) then 0 else n) {
   if (n == 0) then Nil
   else if (n < 0) then Cons((s, t), Cons((s, t), Cons((s, t), Cons((s, t), Cons((s, t), Nil))))) // Ok because norm will remove this
-  else Cons((s, t), dup(n - 1, s, t))
+  else Cons((s, t), dup1(n - 1, s, t))
 }
 
 // CANDIDATE 2
 
-datatype List<T> = Nil | Cons(head: T, tail: List<T>)
-
-
-function dup<S, T>(n: int, s: S, t: T): List<(S, T)>
+function dup2<S, T>(n: int, s: S, t: T): List<(S, T)>
   decreases(if (n <= 0) then 0 else n) {
   if (n <= 0) then Cons((s, t), Nil)
-  else Cons((s, t), dup(n - 1, s, t))
+  else Cons((s, t), dup2(n - 1, s, t))
 }
 
 // CANDIDATE 3
 
-datatype List<T> = Nil | Cons(head: T, tail: List<T>)
-
-
 // Wrong signature
-function dup<S, T>(n: int, t: T, s: S): List<(S, T)>
+function dup3<S, T>(n: int, t: T, s: S): List<(S, T)>
   decreases(if (n <= 0) then 0 else n) {
   if (n <= 0) then Nil
-  else Cons((s, t), dup(n - 1, t, s))
+  else Cons((s, t), dup3(n - 1, t, s))
 }
 
 // CANDIDATE 4
 
-datatype List<T> = Nil | Cons(head: T, tail: List<T>)
-
-
-function dup<S, T>(n: int, s: S, t: T): List<(S, T)>
+function dup4<S, T>(n: int, s: S, t: T): List<(S, T)>
   decreases(if (n <= 0) then 0 else n) {
   if (n <= 0) then Nil
-  else dup(n - 1, s, t) // duplicating nils, very useful
+  else dup4(n - 1, s, t) // duplicating nils, very useful
 }
 
 // CANDIDATE 5
 
-datatype List<T> = Nil | Cons(head: T, tail: List<T>)
-
-function dup<S, T>(n: int, s: S, t: T): List<(S, T)>
+function dup5<S, T>(n: int, s: S, t: T): List<(S, T)>
   decreases(if (n <= 0) then 0 else n) {
   if (n <= 0) then Nil
-  else Cons((s, t), dup(n - 1, s, t))
+  else Cons((s, t), dup5(n - 1, s, t))
 }
 
 
