examples/scalaEquivalenceBenchmarkExamples/max3.dfy
@@ -6,18 +6,18 @@ datatype List<T> = Nil | Cons(head: T, tail: List<T>)
 // but here we ensure that the `choose` functions (created from the `choose((x: int) => true)`)
 // for the Model and the Candidate do not get matched because it would make the type-checker unhappy
 // (because we would create `choose` expressions when doing the replacement).
-function fold(f: (int, int) -> int, l: List<int>, a: int): int
+function foldM(f: (int, int) -> int, l: List<int>, a: int): int
   decreases(l) {
   match l
     case Nil          => a
-    case Cons(hd, tl) => f(hd, fold(f, tl, a))
+    case Cons(hd, tl) => f(hd, foldM(f, tl, a))
   }
 
-ghost function max(lst: List<int>): int {
+ghost function maxM(lst: List<int>): int {
   match lst
     case Nil => var x: int :| true; x
     case Cons(hd, tl) =>
-      fold(
+      foldM(
         (x, y) => if (x > y) then x else y,
         lst,
         hd
@@ -32,21 +32,19 @@ function norm(l: List<int>, f: int): int {
 
 // CANDIDATE
 
-datatype List<T> = Nil | Cons(head: T, tail: List<T>)
-
-function fold(f: (int, int) -> int, l: List<int>, a: int): int
+function fold1(f: (int, int) -> int, l: List<int>, a: int): int
   decreases(l) {
   match l
     case Nil          => a
-    case Cons(hd, tl) => f(hd, fold(f, tl, a))
+    case Cons(hd, tl) => f(hd, fold1(f, tl, a))
 }
 
 // Must be a ghost function since multiple x's can satisfy the such-that assignment
-ghost function max(lst: List<int>): int {
+ghost function max1(lst: List<int>): int {
   match lst
     case Nil => var x: int :| true; x
     case Cons(hd, tl) =>
-      fold(
+      fold1(
         (x, y) => if (x > y) then x else y,
         lst,
         hd
