examples/scalaEquivalenceBenchmarkExamples/separate.dfy
@@ -4,49 +4,41 @@ datatype List<T> = Nil | Cons(head: T, tail: List<T>)
 
 datatype Animal = Sheep(id: int) | Goat(id: int)
 
-function separate(xs: List<Animal>): (List<Animal>, List<Animal>) {
+function separateM(xs: List<Animal>): (List<Animal>, List<Animal>) {
   match xs {
     case Nil => (Nil, Nil)
     case Cons(Sheep(id), t) =>
-      var (s2, g2) := separate(t);
+      var (s2, g2) := separateM(t);
       (Cons(Sheep(id), s2), g2)
     case Cons(Goat(id), t) =>
-      var (s2, g2) := separate(t);
+      var (s2, g2) := separateM(t);
       (s2, Cons(Goat(id), g2))
   }
 }
 
 // CANDIDATE 1
 
-datatype List<T> = Nil | Cons(head: T, tail: List<T>)
-
-datatype Animal = Sheep(id: int) | Goat(id: int)
-
-function separate(xs: List<Animal>): (List<Animal>, List<Animal>) {
+function separate1(xs: List<Animal>): (List<Animal>, List<Animal>) {
   match xs
     case Nil => (Nil, Nil)
     case Cons(Sheep(id), t) =>
-      var (s2, g2) := separate(t);
+      var (s2, g2) := separate1(t);
       (Cons(Sheep(id), s2), g2)
     case Cons(Goat(id), t) =>
-      var (s2, g2) := separate(t);
+      var (s2, g2) := separate1(t);
       (s2, Cons(Goat(id), g2))
   }
 
 // CANDIDATE 2
 
-datatype List<T> = Nil | Cons(head: T, tail: List<T>)
-
-datatype Animal = Sheep(id: int) | Goat(id: int)
-
-function separate(xs: List<Animal>): (List<Animal>, List<Animal>) {
+function separate2(xs: List<Animal>): (List<Animal>, List<Animal>) {
   match xs {
     case Nil => (Nil, Nil)
     case Cons(Sheep(id), t) =>
-      var (s2, g2) := separate(t);
+      var (s2, g2) := separate2(t);
       (Cons(Sheep(id), s2), g2)
     case Cons(Goat(id), t) =>
-      var (s2, g2) := separate(t);
+      var (s2, g2) := separate2(t);
       (s2, g2) // oops, forgets to add goat
   }
 }
