examples/scalaEquivalenceBenchmarkExamples/unknownSafety.dfy
@@ -3,50 +3,48 @@
 datatype List<T> = Nil | Cons(head: T, tail: List<T>)
 
 
-function add(x: int, y: int): int {x + y}
+function addM(x: int, y: int): int {x + y}
 
 /////////////////////////////////////
 
-function isEvenTopLvl(x: int): bool {isEven(x)}
+function isEvenTopLvlM(x: int): bool {isEvenM(x)}
 
-function isEven(x: int): bool
+function isEvenM(x: int): bool
   decreases(if (x <= 0) then 0 else x) {
   if (x < 0) then false
   else if (x == 0) then true
-  else !isOdd(x - 1)
+  else !isOddM(x - 1)
 }
 
-function isOdd(x: int): bool
+function isOddM(x: int): bool
   decreases(if (x <= 0) then 0 else x) {
   if (x <= 0) then false
   else if (x == 1) then true
-  else !isEven(x - 1)
+  else !isEvenM(x - 1)
 }
 
 /////////////////////////////////////
 
-function isSorted(xs: List<int>): bool {
+function isSortedM(xs: List<int>): bool {
   match xs {
   case Nil => true
   case Cons(_, Nil) => true
-  case Cons(h1, Cons(h2, t)) => h1 <= h2 && isSorted(t)
+  case Cons(h1, Cons(h2, t)) => h1 <= h2 && isSortedM(t)
 }
 }
 
 // CANDIDATE
 
-datatype List<T> = Nil | Cons(head: T, tail: List<T>)
 
-
-function zero(x: int): int
+function zero1(x: int): int
   requires (x >= 0) {
-  if (x > 0) then zero(x - 1)
+  if (x > 0) then zero1(x - 1)
   else x
 }
 
-function add(x: int, y: int): int {
+function add1(x: int, y: int): int {
   if (x >= 0) then
-    var z := zero(x);
+    var z := zero1(x);
     assert(z == 0); // timeout
     x + y
   else
@@ -55,40 +53,40 @@ function add(x: int, y: int): int {
 
 /////////////////////////////////////
 
-function isEvenTopLvl(x: int): bool {isEven(x)}
+function isEvenTopLvl1(x: int): bool {isEven1(x)}
 
-function isEven(x: int): bool
+function isEven1(x: int): bool
   decreases(if (x <= 0) then 0 else x) {
   if (x >= 0) then
-    assert(zero(x) == 0); // timeout
+    assert(zero1(x) == 0); // timeout
     if (x < 0) then false
     else if (x == 0) then true
-    else !isOdd(x - 1)
+    else !isOdd1(x - 1)
   else
     if (x < 0) then false
     else if (x == 0) then true
-    else !isOdd(x - 1)
+    else !isOdd1(x - 1)
 }
 
-function isOdd(x: int): bool
+function isOdd1(x: int): bool
   decreases(if (x <= 0) then 0 else x) {
   if (x <= 0) then false
   else if (x == 1) then true
-  else !isEven(x - 1)
+  else !isEven1(x - 1)
 }
 
 /////////////////////////////////////
 
-function isSorted(xs: List<int>): bool {
+function isSorted1(xs: List<int>): bool {
   match xs {
   case Nil => true
   case Cons(h, Nil) =>
     if (h >= 0) then
-      assert(zero(h) == 0); // timeout
+      assert(zero1(h) == 0); // timeout
       true
     else
       true
-  case Cons(h1, Cons(h2, t)) => h1 <= h2 && isSorted(t)
+  case Cons(h1, Cons(h2, t)) => h1 <= h2 && isSorted1(t)
 }
 }
 
