examples/scalaEquivalenceBenchmarkExamples/cloudSculpting.dfy
@@ -2,21 +2,21 @@
 
 // This tests the auxiliary function matching when argument must be permuted to succeed equivalence checking.
 // "cloud scuplting" because does nothing useful (not only that, but also burns fuel...)
-function sculpteurDeNuage<A, B, C>(a: A, b: B, c: C, fuel: int, i1: int, i2: int, i3: int, a2b: A -> B, b2c: B -> C, c2a: C -> A): (int, int, int)
+function sculpteurDeNuageM<A, B, C>(a: A, b: B, c: C, fuel: int, i1: int, i2: int, i3: int, a2b: A -> B, b2c: B -> C, c2a: C -> A): (int, int, int)
   requires (fuel >= 0) {
-  leVraiSculpteurDeNuage(a, b, c, fuel, i1, i2, i3, a2b, b2c, c2a)
+  leVraiSculpteurDeNuageM(a, b, c, fuel, i1, i2, i3, a2b, b2c, c2a)
 }
 
-function leVraiSculpteurDeNuage<A, B, C>(a: A, b: B, c: C, fuel: int, i1: int, i2: int, i3: int, a2b: A -> B, b2c: B -> C, c2a: C -> A): (int, int, int)
+function leVraiSculpteurDeNuageM<A, B, C>(a: A, b: B, c: C, fuel: int, i1: int, i2: int, i3: int, a2b: A -> B, b2c: B -> C, c2a: C -> A): (int, int, int)
   requires (fuel >= 0)
   decreases(fuel) {
   if (fuel == 0) then (i1, i2, i3)
   else
-    var (ii1, ii2, ii3) := mixmash(i1, i2, i3);
-    leVraiSculpteurDeNuage(c2a(c), a2b(a), b2c(b), fuel - 1, ii1, ii2, ii3, a2b, b2c, c2a)
+    var (ii1, ii2, ii3) := mixmashM(i1, i2, i3);
+    leVraiSculpteurDeNuageM(c2a(c), a2b(a), b2c(b), fuel - 1, ii1, ii2, ii3, a2b, b2c, c2a)
 }
 
-function mixmash(i1: int, i2: int, i3: int): (int, int, int) {(i2 - 1, i3 + i2, i1)}
+function mixmashM(i1: int, i2: int, i3: int): (int, int, int) {(i2 - 1, i3 + i2, i1)}
 
 // CANDIDATE
 
